It builds!

BreadBoard/Breadboard.v
@@ -1,103 +1,21 @@
- Require Import String.
- Require Import Ascii.
+Require Import String.
+Require Import Ascii.
 Require Import List.
 Require Import ListSet.
 Require Import EqNat.
 Import ListNotations.
 Require Import Arith.
 Open Scope list_scope.
+Open Scope string_scope.
 
-Notation "$ x" := (fun f => f x) (at level 0, right associativity, only parsing).
-Notation "f $ x .. y" := (.. (f x) .. y) (at level 0, right associativity, only parsing).
-
-
-
-
-
-
-Fixpoint len {T:Type}(x : list T) : nat :=
-  match x with
-    | x::b => 1+len b
-    | nil => 0
-  end.
-Fixpoint suml (x : list nat) : nat :=
-  match x with
-    | x::b => x+suml b
-    | nil => 0
-  end.
-
-Module Wires := Wiring(IO).
+(* Notation "$ x" := (fun f => f x) (at level 0, right associativity, only parsing). *)
+(* Notation "f $ x .. y" := (.. (f x) .. y) (at level 0, right associativity, only parsing). *)
+Require Import Common.
+Require Import IOModule.
+Require Import Run.
+Import IORUN.
 Import Wires.
 
-Module IORUN.
-
-
-  Definition pin_trace_gen w : list (nat* list IO.t):= map (fun p => (p, nil)) (pins w).
-  Search option.
-  Fixpoint find_trace p pt  : option (list IO.t) :=
-    match pt with 
-      | [] => None
-      | (p', t)::rest => if beq_nat p' p then Some t else find_trace p rest 
-    end.
-  Definition find_traces (p :list nat) (pt : list (nat * list IO.t))  : option (list (list IO.t)) :=
-    let elts :=map (fun f =>  (find_trace f pt))  p in
-    let none := forallb (fun x => match x with | None => false | _ => true end ) elts in
-    if none then 
-      Some (map (fun f =>  match f with | None => [] | Some x => x end) elts)
-    else None.
-
-  Definition any_trace  (pt : list (nat * list IO.t) ): list IO.t :=
-    match pt with 
-      | nil => nil
-      | (p', t)::rest => t
-    end.
-  Fixpoint update_trace pt u acc:=
-    match u with
-      | (p, iot)::rest =>
-        match find_trace p pt with
-          | None => update_trace pt rest acc
-          | Some trace =>
-            update_trace pt rest ((p, iot::trace)::acc)
-        end
-      | [] => acc
-    end.
-  Print IO.func.
-  Fixpoint step' w pt (u : list (nat * IO.t))  :=
-    let add_i := set_add in 
-    match w with 
-      | base  =>
-        update_trace pt (u) nil
-      | watch_set w' from (IO.fn_args n fn) to =>
-        let o_traces := (find_traces from pt) in
-        match o_traces with
-          | None => pt
-          | Some traces =>
-            step' w' pt ((to, fn traces )::u)
-        end
-      |  just_set w' (IO.fn_args n fn) to =>
-         step' w' pt  ((to, fn [any_trace  pt ])::u)
-      | join w1 w2 =>
-        app (step' w2 pt [])  (step' w1 pt u)
-      | doc w' _ _ => step' w' pt u
-    end.
-  Definition step w :=
-    step' w (pin_trace_gen w) [].
-
-  Fixpoint run' (w:wiring) (pt: list (nat * list IO.t)) fuel  :=
-    match fuel with
-      | O => pt
-      | S n => run' w (step' w pt []) n
-    end.
-  Definition run w fuel :=
-    run' w (pin_trace_gen w) fuel.
-End IORUN.
-
-
-
-
-
-
-Import IORUN.
 
 (* Module Integrator_Spec. *)
 (*   Definition io (x:list IO.t):IO.t := suml x. *)
@@ -133,151 +51,18 @@ Definition zero_rail   : IO.func := IO.fn_args 0 (fun _ =>0).
 Definition delay_n n default : IO.func := IO.fn_args 1
                                                      (fun x => nth n (hd [] x) default).
 
-Definition p := 1.
-Definition s := "Hello".
-Definition demo1 := base
-                      */  zero_rail ~> 0
-                      //  [5] ~> integrator~> 6
-                      // [2] ~> integrator~> 3
-                      */ incrementor ~> 2
-                      */ IO.fn_args 0 (fun _=> 10) ~> 5
-                      */ alternator ~> 8
-                      # 2 "com".
+
+Open Scope wiring_scope.
+
+Definition demo1 := base */  zero_rail ~> 0
+                         //  [5] ~> integrator~> 6
+                         // [2] ~> integrator~> 3
+                         */ incrementor ~> 2
+                         */ IO.fn_args 0 (fun _=> 10) ~> 5
+                         */ alternator ~> 8
+                         # 2 "com".
 Compute (docstring demo1).
 Definition demo2 := base */integrator ~> 9
                          // [6] ~> delay_n 5 0 ~> 10.
 
-Theorem good_build : valid_wiring (demo1 ~&~ demo2).
-Proof. 
-  autowire.
-Qed.
-
-Theorem bad_build : valid_wiring (demo1 ~&~ demo1) -> False.
-Proof. 
-  autowire.
-Qed.
-
-Compute (find_trace 10 (run (demo1 ~&~ demo2) 10)).
-Theorem no_modify_history_update: forall pin_tr upd n,
-                                    let a := (find_trace n (update_trace pin_tr upd [])) in
-                                    let b := find_trace n pin_tr in
-                                    match (a, b) with
-                                      | (Some (a'::rest), Some rest') =>
-                                        rest = rest'
-                                      | _ => True
-                                    end.
-  intros.
-  unfold a, b. 
-
-  auto.
-  generalize dependent pin_tr.
-
-  induction upd.
-
-  intros.
-
-  induction pin_tr.
-
-  simpl.
-  auto.
-  
-  simpl.
-  auto.
-
-  intros.
-  remember (find_trace n (update_trace pin_tr (a::upd) [] )).
-  destruct o; auto.
-
-  destruct  l; auto.
-
-  remember (find_trace n pin_tr).
-  destruct o; auto.
-
-
-  admit.
-Qed.
-Theorem step_history_safe: forall l w n, 
-                             l = tl (step' w l n).
-  admit.
-Qed.
-
-Theorem no_modify_history: forall n w,  run  w n = tl (run w (S n)).
-Proof.
-  intros.
-
-  induction n.
-  unfold run, run'. 
-  remember (pin_trace_gen w).
-  apply step_history_safe.
-
-  unfold run.
-  
-  remember (pin_trace_gen w).
-  unfold run'.
-  
-  admit.
-  (*  unfold run, run'. *)
-
-  (* apply step_history_safe. *)
-  
-  (*  simpl. *)
-  (*  apply no_modify_history_update. *)
-Qed.
-
-Check no_modify_history.
-Theorem alternates:  forall n, let tr := run demo1 n in
-                               let a :=find_trace 8 tr in
-                               match a with
-                                 | Some ( 0::1::rest)
-                                 | Some (1::0::rest)  => True
-                                 | Some [1] | Some [0] | Some [] => True
-                                 | _ => False
-                                          
-                               end.
-Proof.
-  intros. destruct n.
-  simpl.
-  auto.
-
-  unfold a.
-  unfold tr.
-  unfold run.
-  remember (pin_trace_gen demo1).
-
-  
-  
-  auto.
-  destruct l;auto.
-  simpl.
-  auto.
-
-  admit.
-
-  admit.
-Qed.
-
-(* joined well formed circuits aren't interfered with by an additional module *)
-Theorem non_interference : forall w w', valid_wiring w ->
-                                        valid_wiring  (w ~&~ w') ->
-                                        forall n t,
-                                          let orig := find_trace t (run w n) in
-                                          let mod := find_trace t (run (w ~&~ w') n) in
-                                          match  orig, mod with
-                                            | Some a, Some b => a = b
-                                            | Some a, None => False
-                                            | None, Some a => True
-                                            | None, None => True
-                                          end.
-admit.
-Qed.
-
-(* Funcs are the same*)
-Definition func_same  := forall tr (i i':IO.func),
-                           match i, i' with
-                             |IO.fn_args n f, IO.fn_args n' f'=>
-                              f tr = f' tr /\ n = n'
-                           end.
-
-
-Definition wrapper := IO.func -> IO.func.
 
