BreadBoard/Common.v
@@ -1,4 +1,13 @@
 
+
+Require Import String.
+Require Import Ascii.
+Require Import List.
+Require Import ListSet.
+Require Import EqNat.
+Import ListNotations.
+Require Import Arith.
+Open Scope list_scope.
 Fixpoint len {T:Type}(x : list T) : nat :=
   match x with
     | x::b => 1+len b
