BreadBoard/Theorems.v
@@ -1,0 +1,113 @@
+
+Theorem good_build : valid_wiring (demo1 ~&~ demo2).
+Proof. 
+  autowire.
+Qed.
+
+Theorem bad_build : valid_wiring (demo1 ~&~ demo1) -> False.
+Proof. 
+  autowire.
+Qed.
+
+Compute (find_trace 10 (run (demo1 ~&~ demo2) 10)).
+Theorem no_modify_history_update: forall pin_tr upd n,
+                                    let a := (find_trace n (update_trace pin_tr upd [])) in
+                                    let b := find_trace n pin_tr in
+                                    match (a, b) with
+                                      | (Some (a'::rest), Some rest') =>
+                                        rest = rest'
+                                      | _ => True
+                                    end.
+  intros.
+  unfold a, b. 
+  auto.
+  generalize dependent pin_tr.
+  induction upd.
+  intros.
+  induction pin_tr.
+  simpl.
+  auto.
+  simpl.
+  auto.
+  intros.
+  remember (find_trace n (update_trace pin_tr (a::upd) [] )).
+  destruct o; auto.
+  destruct  l; auto.
+  remember (find_trace n pin_tr).
+  destruct o; auto.
+  admit.
+Qed.
+Theorem step_history_safe: forall l w n, 
+                             l = tl (step' w l n).
+  admit.
+Qed.
+
+Theorem no_modify_history: forall n w,  run  w n = tl (run w (S n)).
+Proof.
+  intros.
+  induction n.
+  unfold run, run'. 
+  remember (pin_trace_gen w).
+  apply step_history_safe.
+  unfold run.
+  remember (pin_trace_gen w).
+  unfold run'.
+  admit.
+  (*  unfold run, run'. *)
+
+  (* apply step_history_safe. *)
+  
+  (*  simpl. *)
+  (*  apply no_modify_history_update. *)
+Qed.
+
+Check no_modify_history.
+Theorem alternates:  forall n, let tr := run demo1 n in
+                               let a :=find_trace 8 tr in
+                               match a with
+                                 | Some ( 0::1::rest)
+                                 | Some (1::0::rest)  => True
+                                 | Some [1] | Some [0] | Some [] => True
+                                 | _ => False
+                                          
+                               end.
+Proof.
+  intros. destruct n.
+  simpl.
+  auto.
+  unfold a.
+  unfold tr.
+  unfold run.
+  remember (pin_trace_gen demo1).
+  auto.
+  destruct l;auto.
+  simpl.
+  auto.
+  admit.
+  admit.
+Qed.
+
+(* joined well formed circuits aren't interfered with by an additional module *)
+Theorem non_interference : forall w w', valid_wiring w ->
+                                        valid_wiring  (w ~&~ w') ->
+                                        forall n t,
+                                          let orig := find_trace t (run w n) in
+                                          let mod := find_trace t (run (w ~&~ w') n) in
+                                          match  orig, mod with
+                                            | Some a, Some b => a = b
+                                            | Some a, None => False
+                                            | None, Some a => True
+                                            | None, None => True
+                                          end.
+admit.
+Qed.
+
+(* Funcs are the same*)
+Definition func_same  := forall tr (i i':IO.func),
+                           match i, i' with
+                             |IO.fn_args n f, IO.fn_args n' f'=>
+                              f tr = f' tr /\ n = n'
+                           end.
+
+
+Definition wrapper := IO.func -> IO.func.
